feat: add support for HPKE (#46)
* feat: add support for HPKE

* hpke: add missing lemmas on `hpke_pk`

* hpke: change key usage from "HPKE" to "DY.Lib.HPKE"

* hpke: use the correct label "base_nonce"

* hpke: add a comment about all the asserts

* hpke: move the "or is publishable" at the end of asserts

* hpke: add more comments around LabeledExpand

* hpke: reorganize `bytes_invariant_aead_enc` precondition

src/core/DY.Core.Bytes.fst
@@ -379,7 +379,7 @@ let get_dh_usage #cusages pk =
 /// this is useful to reason on the corresponding KEM private key label.
 
 [@@"opaque_to_smt"]
-val get_kem_sk_label: {|crypto_usages|} -> bytes -> GTot label
+val get_kem_sk_label: {|crypto_usages|} -> bytes -> label
 let get_kem_sk_label #cusages pk =
   match pk with
   | KemPub sk -> get_label sk
@@ -388,7 +388,7 @@ let get_kem_sk_label #cusages pk =
 /// Same as above, for usage.
 
 [@@"opaque_to_smt"]
-val get_kem_sk_usage: {|crypto_usages|} -> bytes -> GTot usage
+val get_kem_sk_usage: {|crypto_usages|} -> bytes -> usage
 let get_kem_sk_usage #cusages pk =
   match pk with
   | KemPub sk -> get_usage sk
@@ -657,8 +657,7 @@ let rec bytes_invariant #cinvs tr b =
       ) \/ (
         // Attacker case:
         // the attacker knows both prk and info
-        (get_label prk) `can_flow tr` public /\
-        (get_label info) `can_flow tr` public
+        (get_label prk) `can_flow tr` public
       )
     )
   | KemPub sk ->
@@ -1155,8 +1154,14 @@ val bytes_invariant_aead_enc:
     (get_label nonce) `can_flow tr` public /\
     (get_label ad) `can_flow tr` public /\
     (get_label msg) `can_flow tr` (get_label key) /\
-    AeadKey? (get_usage key) /\
-    aead_pred.pred tr key nonce msg ad
+    (
+      (
+        AeadKey? (get_usage key) /\
+        aead_pred.pred tr key nonce msg ad
+      ) \/ (
+        get_label key `can_flow tr` public
+      )
+    )
   )
   (ensures bytes_invariant tr (aead_enc key nonce msg ad))
   [SMTPat (bytes_invariant tr (aead_enc key nonce msg ad))]
@@ -1994,7 +1999,10 @@ val bytes_invariant_kdf_expand:
   (requires
     bytes_invariant tr prk /\
     bytes_invariant tr info /\
-    KdfExpandKey? (get_usage prk)
+    (
+      KdfExpandKey? (get_usage prk) \/
+      get_label prk `can_flow tr` public
+    )
   )
   (ensures bytes_invariant tr (kdf_expand prk info len))
   [SMTPat (bytes_invariant tr (kdf_expand prk info len))]
@@ -2031,6 +2039,22 @@ val get_label_kdf_expand:
 let get_label_kdf_expand prk info len =
   reveal_opaque (`%kdf_expand) (kdf_expand);
   normalize_term_spec get_label
+
+/// User lemma (kdf_expand label can flow)
+
+val get_label_kdf_expand_can_flow:
+  {|crypto_invariants|} ->
+  tr:trace ->
+  prk:bytes -> info:bytes -> len:nat{len <> 0} ->
+  Lemma (get_label (kdf_expand prk info len) `can_flow tr` (get_label prk))
+  [SMTPat (can_flow tr (get_label (kdf_expand prk info len)))]
+let get_label_kdf_expand_can_flow tr prk info len =
+  reveal_opaque (`%kdf_expand) (kdf_expand);
+  normalize_term_spec get_label;
+  match get_usage prk with
+  | KdfExpandKey _ _ ->
+    kdf_expand_usage.get_label_lemma tr (get_usage prk) (get_label prk) info
+  | _ -> ()
 
 (*** KEM ***)
 
@@ -2092,7 +2116,35 @@ let kem_pk_preserves_publishability #ci tr sk =
   normalize_term_spec bytes_invariant;
   normalize_term_spec get_label
 
-/// User lemma (kem_pk usage)
+/// User lemma (kem_pk bytes invariant)
+
+val bytes_invariant_kem_pk:
+  {|crypto_invariants|} ->
+  tr:trace ->
+  sk:bytes ->
+  Lemma
+  (requires bytes_invariant tr sk)
+  (ensures bytes_invariant tr (kem_pk sk))
+  [SMTPat (bytes_invariant tr (kem_pk sk))]
+let bytes_invariant_kem_pk #ci tr sk =
+  normalize_term_spec bytes_invariant;
+  normalize_term_spec kem_pk
+
+/// User lemma (kem_pk sk label)
+
+val get_label_kem_pk:
+  {|crypto_usages|} ->
+  sk:bytes ->
+  Lemma
+  (ensures (
+    get_label (kem_pk sk) == public
+  ))
+  [SMTPat (get_label (kem_pk sk))]
+let get_label_kem_pk #cu sk =
+  normalize_term_spec get_label;
+  normalize_term_spec kem_pk
+
+/// User lemma (kem_pk sk usage)
 
 val get_kem_sk_usage_kem_pk:
   {|crypto_usages|} ->
@@ -2106,7 +2158,7 @@ let get_kem_sk_usage_kem_pk #cu sk =
   normalize_term_spec get_kem_sk_usage;
   normalize_term_spec kem_pk
 
-/// User lemma (kem_pk label)
+/// User lemma (kem_pk sk label)
 
 val get_kem_sk_label_kem_pk:
   {|crypto_usages|} ->
