src/lib/hpke/DY.Lib.HPKE.Lemmas.fst
@@ -1,0 +1,391 @@
+module DY.Lib.HPKE.Lemmas
+
+open Comparse
+open DY.Core
+open DY.Lib.Comparse.Glue
+open DY.Lib.Comparse.Parsers
+open DY.Lib.HPKE.Spec
+open DY.Lib.Crypto.AEAD.Split
+open DY.Lib.Crypto.KdfExpand.Split
+
+#set-options "--fuel 0 --ifuel 1"
+
+/// This module proves security theorems about HPKE, in a modular and reusable way.
+/// The security theorems are similar to the public key encryption ones
+/// (e.g. DY.Core.Bytes.bytes_invariant_pk_dec).
+///
+/// The modularity is achieved using the split invariant mechanism for AEAD and KdfExpand,
+/// allowing for horizontal protocol composition.
+/// The proofs are parametrized by a global HPKE predicate `hpke_crypto_predicate`
+/// (similar to DY.Core.pkenc_crypto_predicate)
+/// which is then compiled to a (local) AEAD predicate (see `hpke_aead_pred`),
+/// allowing for vertical protocol composition.
+///
+/// The proof sketch is the following:
+/// - the shared secret is a KdfExpandKey with usage tag "DY.Lib.HPKE"
+/// - the HPKE usage tag and usage data is serialized into the KdfExpandKey usage data
+///   (using the type `internal_hpke_usage`)
+/// - when the shared secret goes into kdf_expand with `info`,
+///   we obtain an AeadKey with usage tag "DY.Lib.HPKE"
+///   and usage data containing `info` and the HPKE key usage
+///   (using the type `hpke_aead_usage_data`, see `hpke_kdf_expand_usage`)
+/// - when encrypting or decrypting with AEAD,
+///   `plaintext` and `ad` are authenticated by AEAD,
+///   the HPKE usage and `info` are authenticated in the usage data of the AEAD key.
+
+/// Symbolic reduction rule (sanity check)
+
+val hpke_dec_enc:
+  skR:bytes -> entropy:bytes -> plaintext:bytes -> info:bytes -> ad:bytes ->
+  Lemma
+  (hpke_dec skR (hpke_enc (hpke_pk skR) entropy plaintext info ad) info ad == Some plaintext)
+let hpke_dec_enc skR entropy plaintext info ad =
+  FStar.Classical.forall_intro_2 kem_decap_encap;
+  FStar.Classical.forall_intro_4 aead_dec_enc
+
+/// Helper functions to create hpke usages (secret key and entropy)
+
+[@@ with_bytes bytes]
+type internal_hpke_usage = {
+  [@@@ with_parser #bytes ps_string]
+  usage_tag: string;
+  usage_data: bytes;
+}
+
+%splice [ps_internal_hpke_usage] (gen_parser (`internal_hpke_usage))
+
+instance parseable_serializeable_bytes_internal_hpke_usage: parseable_serializeable bytes internal_hpke_usage =
+  mk_parseable_serializeable ps_internal_hpke_usage
+
+val mk_hpke_sk_usage: string & bytes -> usage
+let mk_hpke_sk_usage (usage_tag, usage_data) =
+  KemKey (KdfExpandKey "DY.Lib.HPKE" (serialize _ {usage_tag; usage_data}))
+
+val mk_hpke_entropy_usage: string & bytes -> usage
+let mk_hpke_entropy_usage (usage_tag, usage_data) =
+  KemNonce (KdfExpandKey "DY.Lib.HPKE" (serialize _ {usage_tag; usage_data}))
+
+val mk_hpke_sk_usage_inj:
+  usage1:(string & bytes) -> usage2:(string & bytes) -> 
+  Lemma
+  (requires mk_hpke_sk_usage usage1 == mk_hpke_sk_usage usage2)
+  (ensures usage1 == usage2)
+let mk_hpke_sk_usage_inj (usage_tag1, usage_data1) (usage_tag2, usage_data2) =
+  parse_serialize_inv_lemma #bytes _ { usage_tag = usage_tag1; usage_data = usage_data1 };
+  parse_serialize_inv_lemma #bytes _ { usage_tag = usage_tag2; usage_data = usage_data2 }
+
+/// Obtain the label of the corresponding HPKE private key of a HPKE public key.
+
+val get_hpke_sk_label: {|crypto_usages|} -> bytes -> label
+let get_hpke_sk_label #cusages pk =
+  get_kem_sk_label pk
+
+/// Obtain the usage of the corresponding HPKE private key of a HPKE public key.
+
+val get_hpke_sk_usage: {|crypto_usages|} -> bytes -> usage
+let get_hpke_sk_usage #cusages pk =
+  get_kem_sk_usage pk
+
+/// Type for the HPKE predicate
+
+noeq
+type hpke_crypto_predicate {|crypto_usages|} = {
+  pred: tr:trace -> string & bytes -> msg:bytes -> info:bytes -> ad:bytes -> prop;
+  pred_later:
+    tr1:trace -> tr2:trace ->
+    usage:(string & bytes) -> msg:bytes -> info:bytes -> ad:bytes ->
+    Lemma
+    (requires pred tr1 usage msg info ad /\ tr1 <$ tr2)
+    (ensures pred tr2 usage msg info ad)
+  ;
+}
+
+/// The cryptographic invariants for HPKE.
+
+[@@ with_bytes bytes]
+type hpke_aead_usage_data = {
+  hpke_usg: internal_hpke_usage;
+  info: bytes;
+}
+
+%splice [ps_hpke_aead_usage_data] (gen_parser (`hpke_aead_usage_data))
+
+instance parseable_serializeable_bytes_hpke_aead_usage_data: parseable_serializeable bytes hpke_aead_usage_data =
+  mk_parseable_serializeable ps_hpke_aead_usage_data
+
+let hpke_kdf_expand_usage: kdf_expand_crypto_usage = {
+  get_usage = (fun prk_usage info ->
+    let KdfExpandKey _ data = prk_usage in
+    match parse hpke_labeled_expand_info info, parse internal_hpke_usage data with
+    | Some { len; label = "key"; info }, Some hpke_usg ->
+      AeadKey "DY.Lib.HPKE" (serialize _ { hpke_usg; info; })
+    | Some { len; label = "base_nonce"; info }, Some hpke_usg ->
+      NoUsage // AEAD nonce
+    | _ ->
+      NoUsage
+  );
+  get_label = (fun prk_usage prk_label info ->
+    match parse hpke_labeled_expand_info info with
+    | Some { len; label = "key"; info } ->
+      prk_label
+    | Some { len; label = "base_nonce"; info } ->
+      public
+    | _ ->
+      prk_label
+  );
+  get_label_lemma = (fun tr prk_usage prk_label info -> ());
+}
+
+val hpke_aead_pred: {|cusgs:crypto_usages|} -> hpke_crypto_predicate -> aead_crypto_predicate cusgs
+let hpke_aead_pred #cusgs hpke = {
+  pred = (fun tr key nonce msg ad ->
+    let AeadKey usg data = get_usage key in
+    match parse hpke_aead_usage_data data with
+    | Some { hpke_usg; info; } ->
+      hpke.pred tr (hpke_usg.usage_tag, hpke_usg.usage_data) msg info ad
+    | _ ->
+      False
+  );
+  pred_later = (fun tr1 tr2 key nonce msg ad ->
+    let AeadKey usg data = get_usage key in
+    match parse hpke_aead_usage_data data with
+    | Some { hpke_usg; info; } ->
+      hpke.pred_later tr1 tr2 (hpke_usg.usage_tag, hpke_usg.usage_data) msg info ad
+    | _ -> ()
+  );
+}
+
+/// Integration of the invariants within the split predicate methodology
+
+let hpke_kdf_expand_tag_and_usage = ("DY.Lib.HPKE", hpke_kdf_expand_usage)
+
+val has_hpke_kdf_expand_usage: {|crypto_usages|} -> prop
+let has_hpke_kdf_expand_usage #cu =
+  has_kdf_expand_usage cu hpke_kdf_expand_tag_and_usage
+
+let hpke_aead_tag_and_pred {|crypto_usages|} hpke = ("DY.Lib.HPKE", hpke_aead_pred hpke)
+
+val has_hpke_aead_pred: {|crypto_invariants|} -> hpke_crypto_predicate -> prop
+let has_hpke_aead_pred #cinvs hpke =
+  has_aead_predicate cinvs (hpke_aead_tag_and_pred hpke)
+
+val has_hpke_invariants: {|crypto_invariants|} -> hpke_crypto_predicate -> prop
+let has_hpke_invariants #cinvs hpke =
+  has_hpke_kdf_expand_usage /\
+  has_hpke_aead_pred hpke
+
+/// Lemmas for `hpke_pk`
+
+val bytes_invariant_hpke_pk:
+  {|crypto_invariants|} ->
+  tr:trace ->
+  sk:bytes ->
+  Lemma
+  (requires bytes_invariant tr sk)
+  (ensures bytes_invariant tr (hpke_pk sk))
+  [SMTPat (bytes_invariant tr (hpke_pk sk))]
+let bytes_invariant_hpke_pk #ci tr sk = ()
+
+val get_label_hpke_pk:
+  {|crypto_usages|} ->
+  sk:bytes ->
+  Lemma
+  (ensures get_label (hpke_pk sk) == public)
+  [SMTPat (get_label (hpke_pk sk))]
+let get_label_hpke_pk #cu sk = ()
+
+val get_hpke_sk_usage_hpke_pk:
+  {|crypto_usages|} ->
+  sk:bytes ->
+  Lemma
+  (ensures get_hpke_sk_usage (hpke_pk sk) == get_usage sk)
+  [SMTPat (get_hpke_sk_usage (hpke_pk sk))]
+let get_hpke_sk_usage_hpke_pk #cu sk = ()
+
+val get_hpke_sk_label_hpke_pk:
+  {|crypto_usages|} ->
+  sk:bytes ->
+  Lemma
+  (ensures get_hpke_sk_label (hpke_pk sk) == get_label sk)
+  [SMTPat (get_hpke_sk_label (hpke_pk sk))]
+let get_hpke_sk_label_hpke_pk #cu sk = ()
+
+/// Lemma for `hpke_enc`.
+/// It is a bit more complex than `DY.Core.Bytes.bytes_invariant_pk_enc`,
+/// the additional complexity is explained in the comments.
+
+#push-options "--ifuel 2"
+val bytes_invariant_hpke_enc:
+  {|cinvs:crypto_invariants|} ->
+  hpke:hpke_crypto_predicate ->
+  tr:trace ->
+  pkR:bytes -> entropy:bytes -> msg:bytes -> info:bytes -> ad:bytes ->
+  Lemma
+  (requires
+    is_publishable tr pkR /\
+    bytes_invariant tr entropy /\
+    bytes_invariant tr msg /\
+    bytes_invariant tr info /\
+    is_publishable tr ad /\
+    // the message must flow to the shared secret (derived from the entropy), a requirement of AEAD
+    (get_label msg) `can_flow tr` (get_label entropy) /\
+    // shared secret (derived from the entropy) must flow to the secret key, a requirement of KEM
+    (get_label entropy) `can_flow tr` (get_hpke_sk_label pkR) /\
+    // the entropy and public key must agree on the usage,
+    // or the entropy (hence shared secret) must be publishable:
+    // without this precondition, there could be cross-protocol attacks,
+    // e.g. if a public key of ProtocolA is injected in ProtocolB by the attacker,
+    // then the sender sends a secret to this public key (safe by ProtocolB invariants)
+    // but the receiver expect messages encrypted to this public key to be public (safe by ProtocolA invariants)
+    (
+      (exists usage.
+        get_hpke_sk_usage pkR == mk_hpke_sk_usage usage /\
+        get_usage entropy == mk_hpke_entropy_usage usage
+      ) \/
+      get_label entropy `can_flow tr` public
+    ) /\
+    // but even if it is publishable, the entropy must have a correct usage
+    (exists usage. get_usage entropy == mk_hpke_entropy_usage usage) /\
+    // the HPKE predicate must hold (the `forall` is a way to extract the usage from `pkR`)
+    (forall usage.
+      get_hpke_sk_usage pkR == mk_hpke_sk_usage usage ==>
+      hpke.pred tr usage msg info ad
+    ) /\
+    // the global protocol invariants must contain the HPKE invariants
+    has_hpke_invariants hpke
+  )
+  (ensures (
+    let (enc, ciphertext) = hpke_enc pkR entropy msg info ad in
+    is_publishable tr enc /\
+    is_publishable tr ciphertext
+  ))
+  [SMTPat (hpke_enc pkR entropy msg info ad);
+   SMTPat (bytes_invariant tr msg);
+   SMTPat (has_hpke_invariants hpke);
+  ]
+let bytes_invariant_hpke_enc #cinvs hpke tr pkR entropy msg info ad =
+  eliminate exists usage. get_usage entropy == mk_hpke_entropy_usage usage
+  returns (
+    let (enc, ciphertext) = hpke_enc pkR entropy msg info ad in
+    is_publishable tr enc /\
+    is_publishable tr ciphertext
+  )
+  with _. (
+    let (enc, shared_secret) = kem_encap pkR entropy in
+    bytes_invariant_kem_encap tr pkR entropy;
+    let aead_key = kdf_expand shared_secret (serialize _ { len = 32; label = "key"; info }) 32 in
+    let aead_nonce = kdf_expand shared_secret (serialize _ { len = 32; label = "base_nonce"; info }) 32 in
+
+    let ciphertext = aead_enc aead_key aead_nonce msg ad in
+    assert((enc, ciphertext) == hpke_enc pkR entropy msg info ad);
+    assert(hpke.pred tr usage msg info ad ==> aead_pred.pred tr aead_key aead_nonce msg ad);
+    serialize_wf_lemma _ (bytes_invariant tr) { len = 32; label = "key"; info };
+    serialize_wf_lemma _ (bytes_invariant tr) { len = 32; label = "base_nonce"; info };
+    ()
+  )
+#pop-options
+
+/// HPKE decryption theorem.
+/// It is similar to `DY.Core.Bytes.bytes_invariant_pk_dec`.
+
+#push-options "--ifuel 0"
+val bytes_invariant_hpke_dec:
+  {|cinvs:crypto_invariants|} ->
+  hpke:hpke_crypto_predicate ->
+  tr:trace ->
+  skR:bytes -> enc:bytes -> ciphertext:bytes -> info:bytes -> ad:bytes ->
+  Lemma
+  (requires
+    bytes_invariant tr skR /\
+    (
+      (exists usage. get_usage skR == mk_hpke_sk_usage usage) \/
+      get_label skR `can_flow tr` public
+    ) /\
+    bytes_invariant tr enc /\
+    bytes_invariant tr ciphertext /\
+    bytes_invariant tr info /\
+    bytes_invariant tr ad /\
+    has_hpke_invariants hpke
+  )
+  (ensures (
+    match hpke_dec skR (enc, ciphertext) info ad with
+    | None -> True
+    | Some plaintext ->
+      is_knowable_by (get_label skR) tr plaintext /\
+      (
+        (
+          forall usage. get_hpke_sk_usage (hpke_pk skR) == mk_hpke_sk_usage usage ==>
+          hpke.pred tr usage plaintext info ad
+        ) \/ (
+          is_publishable tr plaintext
+        )
+      )
+  ))
+  [SMTPat (hpke_dec skR (enc, ciphertext) info ad);
+   SMTPat (bytes_invariant tr ciphertext);
+   SMTPat (has_hpke_invariants hpke);
+  ]
+let bytes_invariant_hpke_dec #cinvs hpke tr skR enc ciphertext info ad =
+  let post =
+    match hpke_dec skR (enc, ciphertext) info ad with
+    | None -> True
+    | Some plaintext ->
+      is_knowable_by (get_label skR) tr plaintext /\
+      (
+        (
+          forall usage. get_hpke_sk_usage (hpke_pk skR) == mk_hpke_sk_usage usage ==>
+          hpke.pred tr usage plaintext info ad
+        ) \/ (
+          is_publishable tr plaintext
+        )
+      )
+  in
+
+  let key_info = { len = 32; label = "key"; info } in
+  let key_info_bytes = serialize _ key_info in
+  let nonce_info = { len = 32; label = "base_nonce"; info } in
+  let nonce_info_bytes = serialize _ nonce_info in
+  serialize_wf_lemma _ (bytes_invariant tr) key_info;
+  serialize_wf_lemma _ (bytes_invariant tr) nonce_info;
+
+  eliminate
+    (exists usage. get_usage skR == mk_hpke_sk_usage usage) \/
+    get_label skR `can_flow tr` public
+  returns post
+  with _. (
+    eliminate exists usage. get_usage skR == mk_hpke_sk_usage usage
+    returns _
+    with _. (
+      let (usage_tag, usage_data) = usage in
+      match kem_decap skR enc with
+      | None -> ()
+      | Some shared_secret ->
+        // The `assert`s below are not needed for the proof to work.
+        // They are however useful to debug the proof when tweaking invariants
+        // or tweaking the specification.
+        // This is why we leave these here.
+        assert(bytes_invariant tr shared_secret);
+        assert(get_usage shared_secret == KdfExpandKey "DY.Lib.HPKE" (serialize _ {usage_tag; usage_data}) \/ is_publishable tr shared_secret);
+        let aead_key = kdf_expand shared_secret key_info_bytes 32 in
+        assert(get_usage aead_key == AeadKey "DY.Lib.HPKE" (serialize _ {hpke_usg = {usage_tag; usage_data}; info}) \/ is_publishable tr shared_secret);
+        assert(get_label aead_key == get_label shared_secret \/ is_publishable tr shared_secret);
+        let aead_nonce = kdf_expand shared_secret nonce_info_bytes 32 in
+        assert(get_usage aead_nonce == NoUsage \/ is_publishable tr shared_secret);
+        assert(get_label aead_nonce == public \/ is_publishable tr shared_secret);
+        match aead_dec aead_key aead_nonce ciphertext ad with
+        | None -> ()
+        | Some plaintext -> (
+          assert(get_usage aead_key == AeadKey "DY.Lib.HPKE" (serialize _ { hpke_usg = {usage_tag; usage_data}; info; }) \/ is_publishable tr aead_key);
+          assert(get_usage aead_key == AeadKey "DY.Lib.HPKE" (serialize _ { hpke_usg = {usage_tag; usage_data}; info; }) ==>
+            (aead_pred.pred tr aead_key aead_nonce plaintext ad ==> hpke.pred tr usage plaintext info ad)
+          );
+          FStar.Classical.forall_intro (FStar.Classical.move_requires (mk_hpke_sk_usage_inj usage));
+          ()
+        )
+    )
+  ) and _. (
+    match kem_decap skR enc with
+    | None -> ()
+    | Some shared_secret -> ()
+  )
+#pop-options
